smoke test of conversion

SP1Operations/Compare/LtOperationSigned/Constraints.lean
@@ -6,34 +6,34 @@ namespace LtOperationSigned
 
 section constraints
 
-@[irreducible] def constraints
-  (b : (Word (Fin KB)))
-  (cc : (Word (Fin KB)))
-  (cols : LtOperationSigned)
-  (is_signed : (Fin KB))
-  (is_real : (Fin KB))
-  : SP1ConstraintList (Fin KB) :=
-  let E0 : Fin KB := is_signed - 1
-  let E1 : Fin KB := is_signed * E0
-  let E2 : Fin KB := is_real - 1
-  let E3 : Fin KB := is_real * E2
-  let E4 : Fin KB := is_real - 1
-  let E5 : Fin KB := E4 * is_signed
-  let CS0 : SP1ConstraintList (Fin KB) := U16MSBOperation.constraints b[3] { msb := cols.b_msb.msb } is_signed
-  let CS1 : SP1ConstraintList (Fin KB) := U16MSBOperation.constraints cc[3] { msb := cols.c_msb.msb } is_signed
-  let E6 : Fin KB := is_signed - 1
-  let E7 : Fin KB := E6 * cols.b_msb.msb
-  let E8 : Fin KB := is_signed - 1
-  let E9 : Fin KB := E8 * cols.c_msb.msb
-  let E10 : Fin KB := is_signed * 32768
-  let E11 : Fin KB := b[3] + E10
-  let E12 : Fin KB := 65536 * cols.b_msb.msb
-  let E13 : Fin KB := E11 - E12
-  let E14 : Fin KB := is_signed * 32768
-  let E15 : Fin KB := cc[3] + E14
-  let E16 : Fin KB := 65536 * cols.c_msb.msb
-  let E17 : Fin KB := E15 - E16
-  let CS2 : SP1ConstraintList (Fin KB) := LtOperationUnsigned.constraints #v[b[0], b[1], b[2], E13] #v[cc[0], cc[1], cc[2], E17] { u16_compare_operation := { bit := cols.result.u16_compare_operation.bit }, u16_flags := #v[cols.result.u16_flags[0], cols.result.u16_flags[1], cols.result.u16_flags[2], cols.result.u16_flags[3]], not_eq_inv := cols.result.not_eq_inv, comparison_limbs := #v[cols.result.comparison_limbs[0], cols.result.comparison_limbs[1]] } is_real
+@[irreducible] def constraints {F : Type} [Field F]
+  (b : (Word F))
+  (cc : (Word F))
+  (cols : LtOperationSigned F)
+  (is_signed : F)
+  (is_real : F)
+  : SP1ConstraintList F :=
+  let E0 : F := is_signed - 1
+  let E1 : F := is_signed * E0
+  let E2 : F := is_real - 1
+  let E3 : F := is_real * E2
+  let E4 : F := is_real - 1
+  let E5 : F := E4 * is_signed
+  let CS0 : SP1ConstraintList F := U16MSBOperation.constraints b[3] { msb := cols.b_msb.msb } is_signed
+  let CS1 : SP1ConstraintList F := U16MSBOperation.constraints cc[3] { msb := cols.c_msb.msb } is_signed
+  let E6 : F := is_signed - 1
+  let E7 : F := E6 * cols.b_msb.msb
+  let E8 : F := is_signed - 1
+  let E9 : F := E8 * cols.c_msb.msb
+  let E10 : F := is_signed * 32768
+  let E11 : F := b[3] + E10
+  let E12 : F := 65536 * cols.b_msb.msb
+  let E13 : F := E11 - E12
+  let E14 : F := is_signed * 32768
+  let E15 : F := cc[3] + E14
+  let E16 : F := 65536 * cols.c_msb.msb
+  let E17 : F := E15 - E16
+  let CS2 : SP1ConstraintList F := LtOperationUnsigned.constraints #v[b[0], b[1], b[2], E13] #v[cc[0], cc[1], cc[2], E17] { u16_compare_operation := { bit := cols.result.u16_compare_operation.bit }, u16_flags := #v[cols.result.u16_flags[0], cols.result.u16_flags[1], cols.result.u16_flags[2], cols.result.u16_flags[3]], not_eq_inv := cols.result.not_eq_inv, comparison_limbs := #v[cols.result.comparison_limbs[0], cols.result.comparison_limbs[1]] } is_real
   CS0 ++ CS1 ++ CS2 ++ [
     (.assertZero E1),
     (.assertZero E3),
