SP1Operations/Compare/LtOperationSigned/Operation.lean
@@ -1,7 +1,7 @@
 import SP1Operations.Operation.U16MSBOperation
 import SP1Operations.Compare.LtOperationUnsigned
 
-structure LtOperationSigned where
-  result : LtOperationUnsigned
-  b_msb : U16MSBOperation (Fin KB)
-  c_msb : U16MSBOperation (Fin KB)
+structure LtOperationSigned (F : Type) where
+  result : LtOperationUnsigned F
+  b_msb : U16MSBOperation F
+  c_msb : U16MSBOperation F
