SP1Operations/Compare/LtOperationUnsigned/Constraints.lean
@@ -5,68 +5,68 @@ namespace LtOperationUnsigned
 
 section constraints
 
-@[irreducible] def constraints
-  (b : (Word (Fin KB)))
-  (cc : (Word (Fin KB)))
-  (cols : LtOperationUnsigned)
-  (is_real : (Fin KB))
-  : SP1ConstraintList (Fin KB) :=
-  let E0 : Fin KB := is_real - 1
-  let E1 : Fin KB := is_real * E0
-  let E2 : Fin KB := cols.u16_flags[0] + cols.u16_flags[1]
-  let E3 : Fin KB := E2 + cols.u16_flags[2]
-  let E4 : Fin KB := E3 + cols.u16_flags[3]
-  let E5 : Fin KB := cols.u16_flags[0] - 1
-  let E6 : Fin KB := cols.u16_flags[0] * E5
-  let E7 : Fin KB := cols.u16_flags[1] - 1
-  let E8 : Fin KB := cols.u16_flags[1] * E7
-  let E9 : Fin KB := cols.u16_flags[2] - 1
-  let E10 : Fin KB := cols.u16_flags[2] * E9
-  let E11 : Fin KB := cols.u16_flags[3] - 1
-  let E12 : Fin KB := cols.u16_flags[3] * E11
-  let E13 : Fin KB := E4 - 1
-  let E14 : Fin KB := E4 * E13
-  let E15 : Fin KB := 1 - E4
-  let E16 : Fin KB := 0 + cols.u16_flags[3]
-  let E17 : Fin KB := is_real - E16
-  let E18 : Fin KB := b[3] - cc[3]
-  let E19 : Fin KB := E17 * E18
-  let E20 : Fin KB := b[3] * cols.u16_flags[3]
-  let E21 : Fin KB := 0 + E20
-  let E22 : Fin KB := cc[3] * cols.u16_flags[3]
-  let E23 : Fin KB := 0 + E22
-  let E24 : Fin KB := E16 + cols.u16_flags[2]
-  let E25 : Fin KB := is_real - E24
-  let E26 : Fin KB := b[2] - cc[2]
-  let E27 : Fin KB := E25 * E26
-  let E28 : Fin KB := b[2] * cols.u16_flags[2]
-  let E29 : Fin KB := E21 + E28
-  let E30 : Fin KB := cc[2] * cols.u16_flags[2]
-  let E31 : Fin KB := E23 + E30
-  let E32 : Fin KB := E24 + cols.u16_flags[1]
-  let E33 : Fin KB := is_real - E32
-  let E34 : Fin KB := b[1] - cc[1]
-  let E35 : Fin KB := E33 * E34
-  let E36 : Fin KB := b[1] * cols.u16_flags[1]
-  let E37 : Fin KB := E29 + E36
-  let E38 : Fin KB := cc[1] * cols.u16_flags[1]
-  let E39 : Fin KB := E31 + E38
-  let E40 : Fin KB := E32 + cols.u16_flags[0]
-  let E41 : Fin KB := is_real - E40
-  let E42 : Fin KB := b[0] - cc[0]
-  let E43 : Fin KB := E41 * E42
-  let E44 : Fin KB := b[0] * cols.u16_flags[0]
-  let E45 : Fin KB := E37 + E44
-  let E46 : Fin KB := cc[0] * cols.u16_flags[0]
-  let E47 : Fin KB := E39 + E46
-  let E48 : Fin KB := E45 - cols.comparison_limbs[0]
-  let E49 : Fin KB := E47 - cols.comparison_limbs[1]
-  let E50 : Fin KB := E15 - 1
-  let E51 : Fin KB := cols.comparison_limbs[0] - cols.comparison_limbs[1]
-  let E52 : Fin KB := cols.not_eq_inv * E51
-  let E53 : Fin KB := E52 - is_real
-  let E54 : Fin KB := E50 * E53
-  let CS0 : SP1ConstraintList (Fin KB) := U16CompareOperation.constraints cols.comparison_limbs[0] cols.comparison_limbs[1] { bit := cols.u16_compare_operation.bit } is_real
+@[irreducible] def constraints {F : Type} [Field F]
+  (b : (Word F))
+  (cc : (Word F))
+  (cols : LtOperationUnsigned F)
+  (is_real : F)
+  : SP1ConstraintList F :=
+  let E0 : F := is_real - 1
+  let E1 : F := is_real * E0
+  let E2 : F := cols.u16_flags[0] + cols.u16_flags[1]
+  let E3 : F := E2 + cols.u16_flags[2]
+  let E4 : F := E3 + cols.u16_flags[3]
+  let E5 : F := cols.u16_flags[0] - 1
+  let E6 : F := cols.u16_flags[0] * E5
+  let E7 : F := cols.u16_flags[1] - 1
+  let E8 : F := cols.u16_flags[1] * E7
+  let E9 : F := cols.u16_flags[2] - 1
+  let E10 : F := cols.u16_flags[2] * E9
+  let E11 : F := cols.u16_flags[3] - 1
+  let E12 : F := cols.u16_flags[3] * E11
+  let E13 : F := E4 - 1
+  let E14 : F := E4 * E13
+  let E15 : F := 1 - E4
+  let E16 : F := 0 + cols.u16_flags[3]
+  let E17 : F := is_real - E16
+  let E18 : F := b[3] - cc[3]
+  let E19 : F := E17 * E18
+  let E20 : F := b[3] * cols.u16_flags[3]
+  let E21 : F := 0 + E20
+  let E22 : F := cc[3] * cols.u16_flags[3]
+  let E23 : F := 0 + E22
+  let E24 : F := E16 + cols.u16_flags[2]
+  let E25 : F := is_real - E24
+  let E26 : F := b[2] - cc[2]
+  let E27 : F := E25 * E26
+  let E28 : F := b[2] * cols.u16_flags[2]
+  let E29 : F := E21 + E28
+  let E30 : F := cc[2] * cols.u16_flags[2]
+  let E31 : F := E23 + E30
+  let E32 : F := E24 + cols.u16_flags[1]
+  let E33 : F := is_real - E32
+  let E34 : F := b[1] - cc[1]
+  let E35 : F := E33 * E34
+  let E36 : F := b[1] * cols.u16_flags[1]
+  let E37 : F := E29 + E36
+  let E38 : F := cc[1] * cols.u16_flags[1]
+  let E39 : F := E31 + E38
+  let E40 : F := E32 + cols.u16_flags[0]
+  let E41 : F := is_real - E40
+  let E42 : F := b[0] - cc[0]
+  let E43 : F := E41 * E42
+  let E44 : F := b[0] * cols.u16_flags[0]
+  let E45 : F := E37 + E44
+  let E46 : F := cc[0] * cols.u16_flags[0]
+  let E47 : F := E39 + E46
+  let E48 : F := E45 - cols.comparison_limbs[0]
+  let E49 : F := E47 - cols.comparison_limbs[1]
+  let E50 : F := E15 - 1
+  let E51 : F := cols.comparison_limbs[0] - cols.comparison_limbs[1]
+  let E52 : F := cols.not_eq_inv * E51
+  let E53 : F := E52 - is_real
+  let E54 : F := E50 * E53
+  let CS0 : SP1ConstraintList F := U16CompareOperation.constraints cols.comparison_limbs[0] cols.comparison_limbs[1] { bit := cols.u16_compare_operation.bit } is_real
   CS0 ++ [
     (.assertZero E1),
     (.assertZero E6),
