SP1Operations/Operation/BitwiseU16Operation/Operation.lean
@@ -1,7 +1,7 @@
 import SP1Operations.Operation.U16toU8OperationUnsafe
 import SP1Operations.Operation.BitwiseOperation
 
-@[ext] structure BitwiseU16Operation where
-  b_low_bytes : U16toU8Operation
-  c_low_bytes : U16toU8Operation
-  bitwise_operation : BitwiseOperation
+@[ext] structure BitwiseU16Operation (F : Type) where
+  b_low_bytes : U16toU8Operation F
+  c_low_bytes : U16toU8Operation F
+  bitwise_operation : BitwiseOperation F
