SP1Operations/Operation/U16toU8OperationUnsafe/Operation.lean
@@ -1,4 +1,4 @@
 import SP1Foundations
 
-@[ext] structure U16toU8Operation where
-  low_bytes : Word (Fin KB)
+@[ext] structure U16toU8Operation (F : Type) where
+  low_bytes : Word F
