SP1Operations/Operation/BitwiseOperation/Operation.lean
@@ -1,4 +1,4 @@
 import SP1Foundations
 
-@[ext] structure BitwiseOperation where
-  result : BWord (Fin KB)
+@[ext] structure BitwiseOperation (F : Type) where
+  result : BWord F
