SP1Operations/Operation/MulOperation/Operation.lean
@@ -4,8 +4,8 @@ import SP1Operations.Operation.U16MSBOperation
 @[ext] structure MulOperation where
     carry : Vector (Fin KB) 16
     product : Vector (Fin KB) 16
-    b_lower_byte: U16toU8Operation
-    c_lower_byte: U16toU8Operation
+    b_lower_byte: U16toU8Operation (Fin KB)
+    c_lower_byte: U16toU8Operation (Fin KB)
     b_msb : Fin KB
     c_msb : Fin KB
     product_msb : U16MSBOperation (Fin KB)
